lots of proofs about parents and children getting close to parentheses thm

DFS.v
@@ -894,6 +894,773 @@ Proof.
   intros. pose proof dfs_exec. specialize (X s g o H). destruct X. exists x. apply a.
 Qed.
 
+Lemma pop_stack_app: forall l r,
+  exists l1 l2, 
+  l = l1 ++ l2 /\ pop_stack l r = l2.
+Proof.
+  intros. induction l; simpl.
+  - exists nil. exists nil. split; reflexivity.
+  - destruct a. destruct (S.mem t r) eqn : ?; simpl.
+    + exists nil. exists ((t,o)::l). split; reflexivity.
+    + destruct IHl. destruct H. exists ((t,o) :: x). exists x0.
+      split. simpl. destruct H; rewrite H; reflexivity. destruct H; assumption.
+Qed.
+
+Lemma one_none_in_list: forall (x1: stack) x t o0 s x0,
+(x1 ++ (x, None) :: (t, o0) :: s = x0 ++ (x, None) :: nil /\ forall y : O.t, ~ In (y, None) x0) -> False.
+Proof.
+  intros. destruct H. generalize dependent x1. induction x0; intros; simpl in *.
+  - destruct x1. inversion H. inversion H. destruct x1; inversion H3.
+  - destruct x1; simpl in *. 
+    + inversion H; subst. apply (H0 x). left. reflexivity.
+    + inversion H; subst. eapply IHx0. intros. intro. eapply H0. right. apply H1.
+      apply H3.
+Qed.
+
+Lemma app_inversion: forall (A: Type) (x: A) y l1 l2,
+  l1 ++ (x :: nil) = l2 ++ (y :: nil) ->
+  l1 = l2 /\ x = y.
+Proof.
+  intros. generalize dependent l2. induction l1; intros; subst; simpl in *.
+  - destruct l2. split. reflexivity. inversion H. reflexivity.
+    inversion H. destruct l2; inversion H2.
+  - destruct l2; simpl in H.
+    + inversion H. destruct l1; inversion H2.
+    + inversion H. apply IHl1 in H2. destruct H2; subst; split; reflexivity.
+Qed. 
+
+Lemma app_inversion_2: forall (A: Type) (x:A) l l1 l2,
+  l2 <> nil ->
+  l1 ++ l2 = l ++ (x:: nil) ->
+  exists l3, l2 = l3 ++ (x:: nil).
+Proof.
+  intros. generalize dependent l1. revert l. induction l2; intros; simpl in *.
+  - contradiction.
+  - destruct l1; simpl in *. destruct l; simpl in *. inversion H0; subst. 
+    exists nil. reflexivity. inversion H0; subst. exists (a0 :: l). reflexivity.
+    destruct l; simpl in *. inversion H0; subst.
+     pose proof (app_cons_not_nil l1 l2 a). rewrite H3 in H1. contradiction. inversion H0; subst.
+    destruct l2; simpl in *. apply app_inversion in H3. destruct H3; subst. exists nil. reflexivity.
+    assert (a0 :: l2 <> nil). intro. inversion H1.
+    destruct (IHl2 H1 l ( l1 ++ a ::  nil)). simpl. rewrite <- H3.
+    rewrite <- app_assoc. simpl. reflexivity. exists (a :: x0). rewrite H2. reflexivity.
+Qed.  
+
+Lemma app_inversion_3: forall (A: Type) l1 l2 l3 x (y: A),
+  l1 ++ x :: nil = l2 ++ y :: l3 ->
+  (exists l4, l4 ++ x :: nil = y :: l3).
+Proof.
+  intros. generalize dependent l1. revert l3. induction l2; intros; subst; simpl in *.
+  - exists l1. apply H.
+  - destruct l1; simpl in *.
+    + inversion H. destruct l2; inversion H2.
+    + inversion H; subst. eapply IHl2. apply H2.
+Qed.
+
+Lemma add_to_stack_adds_parent: forall v g r x y,
+  In (x,y) (add_to_stack v g r) ->
+  y = Some v.
+Proof.
+  intros. unfold add_to_stack in H. destruct (G.neighbors_set g v).
+  assert (forall x y l, In (x,y)(fold_right (fun (v0 : S.elt) (t : list (S.elt * option O.t)) => 
+        if S.mem v0 (S.remove v r) then (v0, Some v) :: t else t)
+         nil l) -> y = Some v). { intros. induction l; simpl in H0. destruct H0.
+        destruct (S.mem a (S.remove v r)). simpl in H0. destruct H0. inversion H0. reflexivity. apply IHl.
+        apply H0. apply IHl. apply H0. }
+  eapply H0. apply H. inversion H.
+Qed.
+
+
+Lemma pop_stack_inversion: forall l1 l2 x r y,
+  pop_stack (l1 ++ x :: nil) r = l2 ++ x :: nil ->
+  In y l2 -> In y (pop_stack l1 r).
+Proof.
+  intros. generalize dependent l2. induction l1; intros; simpl in *.
+  - destruct x. destruct (S.mem t r) eqn : ?; simpl in H.
+    + destruct l2. inversion H0. inversion H. destruct l2; inversion H3.
+    + destruct l2; inversion H.
+  - destruct a. destruct (S.mem t r) eqn : ?; simpl in *.
+    + apply (app_inversion _ x x ((t,o) :: l1) l2) in H. destruct H; inversion H; subst.
+      simpl in H0. apply H0.
+    + eapply IHl1. apply H. apply H0.
+Qed.
+
+
+Lemma only_1_root: forall s g o x,
+  valid_dfs_state s g o ->
+  In (x, None) (get_stack s) ->
+  exists l, get_stack s = l ++ (x, None) :: nil /\ forall y, ~In (y, None) l.
+Proof.
+  intros. generalize dependent x. induction H; intros; simpl in *.
+  - destruct o. destruct (G.contains_vertex g v).
+    + simpl in H0. destruct H0. inversion H; subst. exists nil. split. reflexivity.
+      intros. intro. inversion H0. destruct H.
+    + inversion H0.
+    + inversion H0.
+  - inversion H0; subst; simpl in *.
+    + destruct (add_to_stack x0 g0 remain_d) eqn : ?.
+      * simpl in H1. destruct H1. 
+        -- inversion H1; subst. destruct (pop_stack st remain_f) eqn : ?.
+           ++ simpl in H3. destruct (S.min_elt remain_d) eqn : ?.
+              ** inversion H3; subst. exists nil. split. reflexivity. intros. intro. inversion H4.
+              ** inversion H3.
+           ++ simpl in H3. assert (In (x, None) st). eapply in_pop_rev. rewrite Heqs0. inversion H3; subst.
+              left. reflexivity. apply IHvalid_dfs_state in H4. destruct H4. simpl in *.
+              inversion H3; subst. destruct s. exists nil. split. reflexivity. intros. intro. inversion H5.
+              destruct p.
+              pose proof (pop_stack_app st remain_f). destruct H5. destruct H5. destruct H5.
+              rewrite Heqs0 in H6. inversion H6; subst. destruct H4. exfalso. eapply one_none_in_list.
+              split. apply H4. apply H5.
+        -- simpl in *. 
+           destruct (pop_stack st remain_f) eqn : ?; simpl in H3.
+           ++ destruct (S.min_elt remain_d). inversion H3; subst. inversion H1. subst. inversion H3.
+           ++ pose proof (pop_stack_app st remain_f). destruct H4. destruct H4. destruct H4.
+              rewrite Heqs0 in H5. inversion H5; subst. inversion H3; subst. destruct (IHvalid_dfs_state x).
+              apply in_or_app. right. right. apply H1. destruct H4. destruct s; simpl in *.
+              apply app_inversion in H4. destruct H4. inversion H7; subst. exists nil. split.
+              reflexivity. intros. intro. inversion H4. destruct p. destruct H1. inversion H1; subst.
+              destruct s; simpl in *. pose proof (app_inversion _ (x, None) (x, None) (x1 ++ (x0, None) :: nil) (x2)).
+              assert ((x1 ++ (x0, None) :: nil) ++ (x, None) :: nil = x1 ++ (x0, None) :: (x, None) :: nil ).
+              rewrite <- app_assoc. simpl. reflexivity. rewrite H8 in H7. apply H7 in H4. destruct H4.
+              clear H7. clear H8. rewrite <- H4 in H5. exfalso. apply (H5 x0). apply in_or_app.
+              right. left. reflexivity. pose proof app_inversion_2. specialize (H7 _ (x, None) x2
+              (x1 ++ (x0, None) ::(x, None) :: nil) (p::s)). destruct H7.
+              intro. inversion H7. rewrite <- H4. rewrite  <- app_assoc. reflexivity.
+              rewrite H7 in H4. 
+              assert ((x1 ++ (x0, None) :: (x, None) :: x3) ++ (x, None) :: nil = 
+              x1 ++ (x0, None) :: (x, None) :: x3 ++ (x, None) :: nil). rewrite <- app_assoc. reflexivity.  
+                pose proof (app_inversion _ (x, None) (x, None) 
+              (x1 ++ (x0, None) :: (x, None) :: x3) x2). destruct H9. rewrite H8. apply H4. 
+              rewrite <- H9 in H5. exfalso. apply (H5 x0). apply in_or_app. right. left. reflexivity.
+              destruct s; simpl in *. pose proof (app_inversion _ (t, o0) (x, None) (x1 ++ (x0, None) :: nil)
+              x2). destruct H7. rewrite <- app_assoc. rewrite <- H4. reflexivity. 
+              rewrite <- H7 in H5. exfalso. apply (H5 x0). apply in_or_app. right. left. reflexivity.
+              pose proof (app_inversion_2 _ (x, None) x2 (x1 ++ (x0, None) :: (t, o0) :: nil) (p ::s)).
+              destruct H7. intro. inversion H7. rewrite <- H4. rewrite <- app_assoc. reflexivity.
+              rewrite H7 in H4. pose proof (app_inversion _ (x, None) (x, None) (x1 ++ (x0, None) :: (t, o0) :: x3)
+              x2). destruct H8. rewrite <- H4. rewrite <- app_assoc. reflexivity. rewrite <- H8 in H5.
+              exfalso. apply (H5 x0). apply in_or_app. right. left. reflexivity.
+      * simpl in H1. destruct H1. assert (None = Some x0). eapply add_to_stack_adds_parent.
+        rewrite Heqs. rewrite H1. left. reflexivity. inversion H4.
+        apply in_app_or in H1. destruct H1. assert (None = Some x0). eapply add_to_stack_adds_parent.
+        rewrite Heqs. right. apply H1. inversion H4. destruct (pop_stack st remain_f) eqn : ?.
+        -- simpl in H3. destruct (S.min_elt remain_d). inversion H3; subst. simpl in H1.
+           destruct H1. inversion H1; subst. exists (p :: s). split. reflexivity.
+           intros. intro. rewrite <- Heqs in H4. assert (None = Some x). eapply add_to_stack_adds_parent.
+           apply H4. inversion H5. destruct H1. inversion H3.
+        -- simpl in H3. rewrite <- Heqs0 in H3. assert (In (x, None) st). eapply in_pop_rev.
+           rewrite <- H3. apply H1. apply IHvalid_dfs_state in H4. destruct H4. destruct H4.
+           pose proof (pop_stack_app st remain_f). destruct H6. destruct H6. destruct H6.
+           rewrite H4 in H6. subst. rewrite <- H3 in H6. 
+           destruct tl; simpl in *. apply app_inversion in H6. destruct H6. inversion H6; subst.
+           exists (p :: s). split. reflexivity. intros. intro. assert (None = Some x0). eapply
+           add_to_stack_adds_parent. rewrite Heqs. apply H4. inversion H7.
+           pose proof (app_inversion_2 _ (x, None) x1 (x2 ++ (x0, None) :: nil) (p1 :: tl)).
+           destruct H4. intro. inversion H4. rewrite H6. rewrite <- app_assoc. reflexivity.
+           rewrite H4 in H6. pose proof (app_inversion  _ (x, None) (x, None) x1 (x2 ++ (x0, None) :: x3)).
+            destruct H7. rewrite H6. rewrite <- app_assoc. reflexivity. 
+           rewrite H7 in H5. exfalso. apply (H5 x0). apply in_or_app. right. left. reflexivity.
+    + destruct (pop_stack st remain_f) eqn : ?.
+      * simpl in H3. destruct (S.min_elt remain_d); inversion H3.
+      * simpl in H3. rewrite <- H3 in Heqs. apply in_app_or in H1. destruct H1.
+        apply add_to_stack_adds_parent in H1. inversion H1.
+        assert (In (x, None) st). eapply in_pop_rev. rewrite Heqs. apply H1. apply IHvalid_dfs_state in H4.
+        destruct H4. destruct H4. pose proof (pop_stack_app st remain_f). destruct H6. destruct H6.
+        destruct H6. subst. rewrite Heqs in H6. apply app_inversion_3 in H6.
+        destruct H6. exists (add_to_stack x0 g0 remain_d ++ x3). split. rewrite <- app_assoc. rewrite <- H4.
+        reflexivity. intros. intro. apply in_app_or in H6. destruct H6.
+        apply add_to_stack_adds_parent in H6. inversion H6. assert (In (y0, None) x1).
+        rewrite <- H4 in Heqs. 
+        eapply in_pop_rev. eapply pop_stack_inversion in Heqs. apply Heqs. apply H6. 
+        apply (H5 y0). apply H7.
+    + destruct (pop_stack st remain_f) eqn : ?.
+      * simpl in H4. destruct (S.min_elt remain_d). inversion H4; subst. 
+        inversion H1. inversion H4.
+      * simpl in H4. inversion H4; subst. 
+        assert (In (x, None) st). eapply in_pop_rev. rewrite Heqs. simpl. right. apply H1.
+        apply IHvalid_dfs_state in H5. destruct H5. destruct H5. 
+        pose proof (pop_stack_app st remain_f). destruct H7. destruct H7. destruct H7. subst.
+        rewrite Heqs in H7. destruct s; simpl in *. inversion H1.  symmetry in H7.
+        pose proof (app_inversion_2 _ (x, None) x1 (x2 ++ (x0, o0) :: nil) (p :: s)).
+        destruct H5. intro. inversion H5. rewrite <- H7. rewrite <- app_assoc. reflexivity.
+        exists x3. split. apply H5. rewrite H5 in H7. pose proof (app_inversion _ (x, None)
+        (x, None) x1 (x2 ++ (x0, o0) :: x3)). destruct H8. rewrite <- H7. rewrite <- app_assoc.
+        reflexivity. intros. intro. rewrite H8 in H6. apply (H6 y). apply in_or_app. right. right.
+        apply H10.
+Qed. 
+
+Lemma stack_elt_dec: forall (x y: O.t * option O.t),
+  {x = y} + {x <> y}.
+Proof.
+decide equality.  subst. destruct b. destruct o.
+destruct (O.eq_dec t0 t1). rewrite e. left. reflexivity.
+right. intro. inversion H; subst. apply n. reflexivity.
+right. intro. inversion H.
+destruct o. right. intro. inversion H.
+left. reflexivity. simpl in *.
+apply O.eq_dec.
+Qed.
+
+Lemma in_split_list: forall (l: stack) x,
+  (exists y, In (x, y) l) ->
+  exists l1 l2 y, l1 ++ (x, y) :: l2 = l /\ forall y', ~In (x, y') l1.
+Proof.
+  intros. induction l.
+  - destruct H. inversion H.
+  - simpl in H. destruct H.  destruct a. destruct (O.eq_dec t x).
+    + unfold O.eq in e. subst. destruct H.
+      * inversion H; subst. exists nil. exists l. exists x0. split. reflexivity.
+        intros. intro. inversion H0.
+      * exists nil. exists l. exists o. split. reflexivity. intros. intro. inversion H0.
+    + destruct H. inversion H; subst. exfalso. apply n. reflexivity. destruct IHl.
+      exists x0. apply H. destruct H0. destruct H0. destruct H0. rewrite <- H0.
+      exists ((t, o) :: x1). exists x2. exists x3. split. reflexivity. intros. intro.
+      destruct H2. inversion H2; subst. apply n. reflexivity. apply (H1 y'). apply H2.
+Qed.
+
+
+Lemma gray_list: forall s g o v,
+  valid_dfs_state s g o ->
+  gray s v = true ->
+  exists l1 l2 p, l1 ++ (v, p) :: l2 = get_stack s /\ forall p', ~In (v, p') l1.
+Proof.
+  intros. eapply gray_on_stack in H0. destruct H0. destruct (in_split_list (get_stack s) v).
+  exists x. apply H0. exists x0. apply H1. apply H.
+Qed. 
+
+Lemma only_add_yet_to_be_discovered: forall v g r x y,
+  In (x,y) (add_to_stack v g r) ->
+  S.mem x r = true.
+Proof.
+  intros. unfold add_to_stack in H. destruct (G.neighbors_set g v).
+  assert (forall x y l, In (x, y)
+      (fold_right
+         (fun (v0 : S.elt) (t : list (S.elt * option O.t)) =>
+          if S.mem v0 (S.remove v r) then (v0, Some v) :: t else t) nil l) -> S.mem x r = true). { 
+  intros. induction l; simpl in H0. destruct H0. destruct (S.mem a (S.remove v r) )eqn : ?.
+        simpl in H0. destruct H0. inversion H0; subst. rewrite P2.Dec.F.remove_b in Heqb.
+        rewrite andb_true_iff in Heqb. destruct Heqb. apply H1.
+ all: apply IHl; apply H0. }
+  eapply H0. apply H. inversion H.
+Qed.
+
+Lemma add_to_stack_neq: forall v g r x y,
+  In (x,y) (add_to_stack v g r) ->
+  x <> v.
+Proof.
+  intros. unfold add_to_stack in H. destruct (G.neighbors_set g v) eqn : ?.
+  - assert (forall x y l, In (x,y)(fold_right
+         (fun (v0 : S.elt) (t : list (S.elt * option O.t)) =>
+          if S.mem v0 (S.remove v r) then (v0, Some v) :: t else t) nil l) -> x <> v). {
+  intros. induction l. simpl in H0. destruct H0. simpl in H0.
+  destruct (S.mem a (S.remove v r)) eqn : ?. simpl in H0. destruct H0.
+  inversion H0; subst. intro; subst. rewrite P2.Dec.F.remove_b in Heqb.
+  rewrite andb_true_iff in Heqb. destruct Heqb. unfold P2.Dec.F.eqb in H2.
+  destruct (O.eq_dec v v ). inversion H2. apply n. apply eq_refl.
+  apply IHl. apply H0. apply IHl. apply H0. } eapply H0.
+  apply H.
+  - inversion H.
+Qed.
+
+Lemma parents_not_white: forall s g o x y,
+  valid_dfs_state s g o ->
+  In (x, Some y) (get_stack s) ->
+  white s y = false.
+Proof.
+  intros. unfold white. induction H; subst; simpl in *.
+  - destruct o. destruct (G.contains_vertex g v). inversion H0. inversion H. inversion H. inversion H0.
+    inversion H0.
+  - inversion H1; subst; simpl in *.
+    + simplify. apply in_app_or in H0. destruct H0.
+      * apply add_to_stack_adds_parent in H0. inversion H0; subst. left. 
+        destruct (S.mem x0 (S.remove x0 remain_d)) eqn : ?. exfalso. eapply remove_eq. apply Heqb. reflexivity.
+      * destruct (pop_stack st remain_f) eqn : ?.
+        -- simpl in H3. destruct (S.min_elt remain_d); inversion H3; subst. simpl in H0.
+           destruct H0; inversion H0.
+        -- simpl in H3. rewrite <-  H3 in Heqs. destruct IHvalid_dfs_state. eapply in_pop_rev. rewrite Heqs. apply H0.
+           left. rewrite P2.FM.remove_b. simplify. right. apply H4.
+   + simplify. apply in_app_or in H0. destruct H0.
+      * apply add_to_stack_adds_parent in H0. inversion H0; subst. left. 
+        destruct (S.mem x0 (S.remove x0 remain_d)) eqn : ?. exfalso. eapply remove_eq. apply Heqb. reflexivity.
+      * destruct (pop_stack st remain_f) eqn : ?.
+        -- simpl in H3. destruct (S.min_elt remain_d); inversion H3; subst. 
+        -- simpl in H3. rewrite <-  H3 in Heqs. destruct IHvalid_dfs_state. eapply in_pop_rev. rewrite Heqs. apply H0.
+           destruct (O.eq_dec x0 y). rewrite e in H2. rewrite H2 in H4. inversion H4. 
+           left. rewrite P2.FM.remove_b. simplify. right. apply H4.
+    + simplify. destruct (pop_stack st remain_f) eqn : ?.
+      * simpl in H4. destruct (S.min_elt remain_d); inversion H4; subst. inversion H0.
+      * simpl in H4. rewrite <- H4 in Heqs. destruct IHvalid_dfs_state.
+        eapply in_pop_rev. rewrite Heqs. right. apply H0.
+        left. apply H5. right. rewrite P2.FM.remove_b. simplify.
+Qed.
+
+Lemma root_nil: forall s g o v l tl,
+  valid_dfs_state s g o ->
+  get_stack s = l ++ (v, None) :: tl ->
+  tl = nil.
+Proof.
+  intros. pose proof only_1_root. specialize (H1 s g o v H). destruct H1.
+  - rewrite H0. apply in_or_app. right. left. reflexivity.
+  - destruct tl. reflexivity. destruct H1. rewrite H1 in H0.
+    pose proof (app_inversion_2 _ (v, None) x (l ++ (v, None) :: nil) (p :: tl)). destruct H3.
+    intro. inversion H3. rewrite H0. rewrite <- app_assoc. reflexivity. rewrite H3 in H0.
+    pose proof (app_inversion _ (v, None) (v, None) x (l ++ (v, None) :: x0)). destruct H4.
+    rewrite H0. rewrite <- app_assoc. reflexivity. rewrite H4 in H2. exfalso. apply (H2 v).
+    apply in_or_app. right. left. reflexivity.
+Qed. 
+
+Lemma pair_neq_add_to_stack: forall v g r x y,
+  In (x, Some y) (add_to_stack v g r) ->
+  x <> y.
+Proof.
+  intros. unfold add_to_stack in H. assert (forall x y l,
+  In (x, Some y) (fold_right
+            (fun (v0 : S.elt) (t : list (S.elt * option O.t)) =>
+             if S.mem v0 (S.remove v r) then (v0, Some v) :: t else t) nil l )->  x <> y).
+{ intros. induction l. simpl in H0. destruct H0. simpl in H0. destruct (S.mem a (S.remove v r)) eqn : ?.
+  simpl in H0. destruct H0. inversion H0; subst. intro. subst. eapply remove_eq. apply Heqb.
+  apply IHl; assumption. apply IHl; assumption. }
+  destruct (G.neighbors_set g v). eapply H0. apply H. inversion H.
+Qed.
+
+Lemma neq_parent: forall s g o x y,
+  valid_dfs_state s g o ->
+  In (x, Some y) (get_stack s) ->
+  x <> y.
+Proof.
+  intros. induction H; subst; simpl in *.
+  - destruct o. destruct (G.contains_vertex g v). inversion H0. inversion H. inversion H.
+    inversion H0. inversion H0. 
+  - inversion H1; subst; simpl in *.
+    + apply in_app_or in H0. destruct H0.
+      * apply pair_neq_add_to_stack in H0. assumption.
+      * destruct (pop_stack st remain_f) eqn : ?; simpl in H3. destruct (S.min_elt remain_d); inversion H3; subst.
+        simpl in H0. destruct H0; inversion H0. apply IHvalid_dfs_state. eapply in_pop_rev. rewrite Heqs.
+        rewrite <- H3. apply H0.
+    + apply in_app_or in H0. destruct H0.
+      * apply pair_neq_add_to_stack in H0. assumption.
+      * destruct (pop_stack st remain_f) eqn : ?; simpl in H3. destruct (S.min_elt remain_d); inversion H3; subst.
+         apply IHvalid_dfs_state. eapply in_pop_rev. rewrite Heqs.
+        rewrite <- H3. apply H0.
+    + destruct (pop_stack st remain_f) eqn : ?; simpl in H4. destruct (S.min_elt remain_d); inversion H4; subst.
+      destruct H0. apply IHvalid_dfs_state. eapply in_pop_rev. rewrite Heqs. rewrite <- H4. right. apply H0.
+Qed.
+
+Inductive dfs_multi_alt : state -> state -> Prop :=
+  | refl': forall s, dfs_multi_alt s s
+  | step': forall s1 s2 s3, dfs_multi_alt s1 s2 -> dfs_step s2 s3 -> dfs_multi_alt s1 s3.
+
+Lemma multi_alt_trans: forall s s' s'',
+  dfs_multi_alt s s' ->
+  dfs_multi_alt s' s'' ->
+  dfs_multi_alt s s''.
+Proof.
+  intros. induction H0.
+  - assumption.
+  - eapply step'. apply IHdfs_multi_alt. apply H. apply H1.
+Qed. 
+
+Lemma multi_equiv: forall s s',
+  dfs_multi s s' <-> dfs_multi_alt s s'.
+Proof.
+  intros. split; intros; induction H.
+  - apply refl'.
+  - eapply multi_alt_trans. eapply step'. apply refl'. apply H. apply IHmulti.
+  - apply multi_refl.
+  - eapply multi_trans. apply IHdfs_multi_alt. apply multi_R. apply H0.
+Qed.
+
+Lemma pop_stack_delete: forall s r a b,
+  In (a,b) s ->
+  S.mem a r = false \/ In (a,b) (pop_stack s r).
+Proof.
+  intros. induction s.
+  - inversion H.
+  - simpl in *. destruct a0. destruct H.
+    + inversion H; subst. destruct (S.mem a r) eqn : ?.
+      * simpl. right. left. reflexivity.
+      * simpl. left. reflexivity.
+    + destruct (S.mem a r) eqn : ?; simpl.
+      * right. destruct (S.mem e r) eqn : ?; simpl.
+        -- right. apply H.
+        -- apply IHs in H. destruct H. inversion H. apply H.
+      * left. reflexivity.
+Qed.
+
+Lemma list_cons_neq: forall (A: Type) (x: A) l,
+  l <> x :: l.
+Proof.
+  intros. induction l. intro. inversion H.
+  intro. inversion H. contradiction.
+Qed.
+
+Lemma list_app_neq: forall (A: Type) (l l1: list A),
+  l1 <> nil ->
+  l <> l1 ++ l.
+Proof.
+  intros. generalize dependent l1. induction l; intros; simpl in *.
+  - destruct l1. contradiction. intro. inversion H0.
+  - intro. destruct l1. contradiction. inversion H0; subst. eapply IHl. 
+    assert (l1 ++ (a0:: nil) <> nil). intro. destruct l1; inversion H1. apply H1.
+    rewrite H3 at 1. rewrite <- app_assoc. reflexivity.
+Qed.
+
+Lemma pop_no_app: forall l l1 r,
+  l1 <> nil ->
+  pop_stack l r <> l1 ++ l.
+Proof.
+  intros. generalize dependent l1. induction l; intros; simpl in *.
+  + destruct l1. contradiction. intro. inversion H0.
+  + destruct a. destruct (S.mem t r); simpl in *.
+    - intro. destruct l1. contradiction.
+      inversion H0; subst. eapply list_app_neq.
+      assert (l1 ++ (t,o):: nil <> nil). intro. destruct l1; inversion H1.
+      apply H1. rewrite <- app_assoc. apply H3.
+    - intro. assert (l1 ++ (t,o) :: l = l1 ++ (t,o) :: nil ++ l). simpl. reflexivity.
+      rewrite H1 in H0. eapply IHl. 
+      assert (l1 ++ (t,o) :: nil <> nil). intro. destruct l1; inversion H2.
+      apply H2. rewrite <- app_assoc. apply H0.
+Qed.
+
+Lemma pop_no_add: forall x l r,
+  pop_stack l r <> x :: l.
+Proof.
+  intros. assert (x :: l = x :: nil ++ l). simpl. reflexivity. rewrite H.
+  intro. eapply pop_no_app. assert (x :: nil <> nil). intro. inversion H1.
+  apply H1. simpl. apply H0.
+Qed.
+
+
+Lemma pop_stack_app_distr: forall l1 l2 a b r,
+   S.mem a r = true -> pop_stack (l1 ++ (a,b) :: l2) r = (pop_stack l1 r) ++ ((a,b) :: l2).
+Proof.
+  intros. generalize dependent l2. induction l1; subst; intros.
+    + simpl. rewrite H. simpl. reflexivity.
+    + simpl in *. destruct a0. destruct (S.mem e r) eqn : ?; simpl. reflexivity.
+      apply IHl1.
+Qed. 
+
+(*An important lemma: The stack to the left of a gray vertex does not change. Moreover,
+  the rest of the stack does not contain v, and the previous does not have v as a parent.
+  This is key to proving that the search proceeds in a depth first manner*)
+(*TODO: may want to add that o' is parent in forest (or if none then it is root)*)
+Lemma right_left_stacks: forall s g o v,
+  valid_dfs_state s g o ->
+  exists tl o',
+  gray s v = true ->
+  (exists l1, get_stack s = l1 ++ (v,o') :: tl /\ (forall o'', ~In (v, o'') l1) /\
+  (forall y, ~In (y, Some v) tl)).
+Proof.
+  intros. unfold gray in *. induction H; subst; simpl in *.
+  - destruct o. destruct (G.contains_vertex g v0) eqn : ?.
+    + exists nil. exists None. intros. simplify. rewrite H1 in H0. inversion H0.
+    + exists nil. exists None. intros. simplify. rewrite H1 in H0. inversion H0.
+    + exists nil. exists None. intros. simplify. rewrite H1 in H0. inversion H0.
+  - inversion H0; subst; simpl in *; destruct IHvalid_dfs_state.
+    + destruct H3. assert (tl = nil). eapply root_nil. eapply step. apply H. apply H0. simpl. reflexivity.
+    subst. destruct (O.eq_dec x v). 
+      * unfold O.eq in e. subst. exists nil. exists None. intros. exists (add_to_stack v g0 remain_d).
+        split. reflexivity. intros. split. intros. intro. apply add_to_stack_neq in H5. contradiction.
+        intros. intro. inversion H5.
+      * (*doesn't matter, this is impossible*)
+        exists nil. exists None. intros. remember (g0, f, f_times, d_times, time, remain_d, remain_f, st) as s.
+       assert (exists o, In (v, o) (get_stack s)). eapply gray_on_stack. apply H.
+       unfold gray; subst; simpl in *. simplify. rewrite P2.FM.remove_neq_b in H5. apply H5. intuition.
+       subst; simpl in *. destruct H5. destruct (pop_stack st remain_f) eqn : ?.
+       -- simpl in H2. rewrite pop_stack_nil in Heqs. specialize (Heqs (v, x2)).
+          simpl in Heqs. apply Heqs in H5. simplify. rewrite H5 in H7. inversion H7.
+       -- simpl in H2. inversion H2; subst. eapply (pop_stack_delete _ remain_f) in H5.
+          destruct H5. simplify. rewrite H7 in H5. inversion H5.
+          rewrite Heqs in H5. simpl in H5. destruct H5. inversion H5. subst. simplify. exfalso. apply n.
+          reflexivity. destruct H5.
+    + destruct H3. destruct (O.eq_dec x v).
+      * exists tl. exists (Some y). intros. exists (add_to_stack x g0 remain_d). split. 
+        rewrite e. reflexivity. intros. split. intros. intro. apply add_to_stack_neq in H5. rewrite e in H5.
+        contradiction. intros. intro. rewrite e in H1. 
+        remember (g0, t :: f, f_times, d_times, time, remain_d, remain_f, st) as s.
+        assert (white s v = true). unfold white; subst; simpl; simplify.
+        pose proof parents_not_white. specialize (H7 s g o y0 v). apply H7 in H. rewrite H in H6. inversion H6.
+         subst; simpl. destruct (pop_stack st remain_f) eqn : ?.
+        -- simpl in H2. destruct (S.min_elt remain_d). inversion H2; subst. inversion H2.
+        -- simpl in H2. rewrite <- H2 in Heqs. eapply in_pop_rev. rewrite Heqs. right. apply H5.
+      * exists x0. exists x1. intros. destruct H3.
+        rewrite P2.FM.remove_neq_b in H4. apply H4. apply n.
+        destruct (pop_stack st) eqn : ?.
+        -- simpl in H2. destruct (S.min_elt remain_d); inversion H2.
+        -- simpl in H2. exists (add_to_stack x g0 remain_d ++ (pop_stack (x2) remain_f)).
+        split. destruct H3. rewrite H2. rewrite <- Heqs. rewrite H3. rewrite pop_stack_app_distr.
+        rewrite app_assoc. reflexivity. simplify. split. intros. intro. apply in_app_or in H5.
+        destruct H5. apply only_add_yet_to_be_discovered in H5. simplify.
+        rewrite P2.FM.remove_neq_b in H6. rewrite H6 in H5. inversion H5. intuition. 
+        destruct H3. destruct H6. apply (H6 o''). eapply in_pop_rev. apply H5.
+        intros. intro. destruct H3. destruct H6. apply (H7 y0). apply H5.
+    + destruct H4. destruct (O.eq_dec x v).
+      * unfold O.eq in e. subst. destruct H4. simplify. destruct H4.
+        exists x0. exists x1. intros. simplify. exfalso. eapply remove_eq. apply H9.
+      * exists x0. exists x1. intros. simplify.
+        rewrite P2.FM.remove_neq_b in H7. destruct H4. assumption.
+        destruct (pop_stack st remain_f) eqn : ?.
+        -- simpl in H3. destruct (S.min_elt remain_d) eqn : ?; inversion H3; subst.
+           remember (g0, f, M.add e (time + 1) f_times, d_times, time + 1, remain_d, S.remove e remain_f, nil) as s.
+           assert (exists o, In (v,o) (get_stack s)). eapply gray_on_stack. eapply step. apply H.
+           apply H0. unfold gray. subst; simpl; simplify. subst; simpl in *. destruct H5. destruct H5.
+        -- simpl in H3. rewrite <- H3 in Heqs.
+            destruct H4. rewrite H4 in Heqs. rewrite pop_stack_app_distr in Heqs.
+            destruct (pop_stack x2 remain_f) eqn : ?.
+            ++ inversion Heqs; subst. exfalso. apply n. reflexivity.
+            ++ inversion Heqs; subst. exists s0. split. reflexivity. split. intros.
+               destruct H5.
+               apply (H5 o''). eapply in_pop_rev. rewrite Heqs0. right. apply H4.
+                destruct H5. apply H5.
+            ++ apply H7.
+       -- intuition.
+Qed. 
+
+
+(*
+Lemma proper_stack: forall s g o v o' tl,
+  valid_dfs_state s g o ->
+  get_stack s = (v, o') :: tl ->
+  white s v = true ->
+  (forall s', dfs_multi s s' ->
+    gray s' v = true ->
+    exists l1, get_stack s' = l1 ++ (v, o') :: tl /\ (forall o'', ~In (v, o'') l1)).
+Proof.
+  intros. assert (valid_dfs_state s' g o). eapply multistep_preserves_valid. apply H. apply H2.
+   eapply right_left_stacks in H4. destruct H4. destruct H4. apply H4 in H3. destruct H3.
+    unfold gray in *; unfold white in *. induction H2.
+  - simplify. rewrite H2 in H1. inversion H1.
+  - inversion H2; subst; simpl in *.
+    + 
+
+
+   unfold whit 
+*)
+
+Lemma destruct_app: forall (l1: stack) x l2 y  l3,
+  l1 ++ x :: l2 = y :: l3 ->
+  (l1 = nil /\ x = y /\ l2 = l3) \/ In y l1.
+Proof.
+  intros. induction l1.
+  - simpl in H. inversion H; subst. left. split; try(split); reflexivity.
+  - destruct (stack_elt_dec y a).
+    + subst. right. simpl. left. reflexivity.
+    + inversion H; subst. contradiction.
+Qed.  
+
+Lemma parent_gray: forall s g o y,
+  valid_dfs_state s g o ->
+  (exists x, In (x, Some y) (get_stack s)) ->
+  gray s y = true.
+Proof.
+  intros. unfold gray. induction H; subst; simpl in *.
+  - destruct o. destruct (G.contains_vertex g v). all: repeat(try(inversion H); try(inversion H0); try(inversion H1)).
+  - inversion H1; subst; simpl in *.
+    + assert (tl = nil). remember (g0, T.singleton x :: f, f_times, M.add x (time + 1) d_times, time + 1, S.remove x remain_d, remain_f,
+       add_to_stack x g0 remain_d ++ (x, None) :: tl) as s.
+      eapply root_nil. eapply step. apply H. apply H1. subst; simpl. reflexivity. subst.
+      destruct H0. apply in_app_or in H0. destruct H0.
+      * apply add_to_stack_adds_parent in H0. inversion H0; subst. simplify.
+        destruct (S.mem x (S.remove x remain_d)) eqn : ?. exfalso. eapply remove_eq. apply Heqb.
+        reflexivity. remember (g0, f, f_times, d_times, time, remain_d, remain_f, st) as s.
+        assert (S.mem x (get_remain_d s ) = true) by (subst; simpl; assumption). 
+        eapply not_f_if_not_d in H4. subst; simpl in *; assumption. apply H.
+      * simpl in H0; destruct H0; inversion H0.
+    + destruct H0. apply in_app_or in H0. destruct H0. apply add_to_stack_adds_parent in H0. inversion H0; subst.
+      simplify. destruct (S.mem x (S.remove x remain_d)) eqn : ?. exfalso. eapply remove_eq. apply Heqb. reflexivity.
+      remember (g0, t :: f, f_times, d_times, time, remain_d, remain_f, st) as s.
+      assert (S.mem x (get_remain_d s) = true) by (subst; simpl; assumption). eapply not_f_if_not_d in H4.
+      subst; simpl in *; assumption. apply H. destruct (pop_stack st remain_f) eqn : ?; simpl in H3.
+      * destruct (S.min_elt remain_d); inversion H3; subst.
+      * rewrite andb_true_iff. assert (exists x, In (x, Some y) st). exists x0. eapply in_pop_rev.
+        rewrite Heqs. rewrite <- H3. apply H0. apply IHvalid_dfs_state in H4. split. simplify.
+        rewrite P2.Dec.F.remove_b. simplify. simplify.
+    + destruct H0. (*ugh, need to know that if we are remvoving this, then there are none in the end*)
+      destruct (O.eq_dec x y).
+      * remember (g0, f, f_times, d_times, time, remain_d, remain_f, st) as s.
+        assert (gray s x = true). subst; unfold gray; simpl in *; simplify.
+        pose proof (right_left_stacks  s g o x H). destruct H6. destruct H6. 
+        apply H6 in H5. clear H6. destruct H5. destruct H5. subst; simpl in *.
+        destruct (pop_stack st remain_f) eqn : ?.
+        -- simpl in H4. destruct (S.min_elt remain_d). inversion H4; subst. destruct H0.
+            inversion H4.
+        -- simpl in H4. rewrite <- H4 in Heqs. rewrite H5 in Heqs. 
+           rewrite pop_stack_app_distr in Heqs. destruct H6. 
+           pose proof destruct_app. specialize (H8 (pop_stack x3 remain_f) (x, x2) x1 (x, o0) tl).
+           apply H8 in Heqs. assert (In (x0, Some y) x1). { destruct Heqs.
+           ++ destruct H9. destruct H10. inversion H10; subst. apply H0.
+           ++ assert (In (x, o0) x3). eapply in_pop_rev. apply H9. exfalso. apply (H6 o0).
+              apply H10. } exfalso. apply (H7 x0). rewrite e. apply H9. apply H3.
+      * destruct (pop_stack st remain_f) eqn : ?.
+        ++ simpl in H4. destruct (S.min_elt remain_d); inversion H4; subst. destruct H0.
+        ++ simpl in H4. rewrite <- H4 in Heqs. assert (exists x, In (x, Some y) st). exists x0. eapply in_pop_rev.
+           rewrite Heqs. right. apply H0. apply IHvalid_dfs_state in H5. simplify.
+Qed.
+
+Lemma parent_gray_when_child_active: forall s g o x y,
+  valid_dfs_state s g o ->
+  In (x, Some y) (get_stack s) ->
+  gray s x = true ->
+  gray s y = true.
+Proof.
+  intros. eapply parent_gray. apply H. exists x. apply H0.
+Qed.
+
+
+(*Let's prove a stronger version of this
+If (x, Some y) is on the stack and x is gray, then y is gray - did even better - if (x,y) is on the stack,
+  then y is gray  q*)
+(*Then prove: If x -> y is in the tree, then (x, Some y) is on the stack*)
+
+(*
+Lemma tree_not_white: forall s g o v,
+  valid_dfs_state s g o ->
+  G.contains_vertex g v = true ->
+  (exists t f, get_forest s = t :: f /\ T.contains_vertex t v = true) <-> white s v = false.
+Proof.
+  intros. unfold white. induction H; subst; simpl in *; split; intros.
+  - destruct H. destruct H. destruct H. inversion H.
+  - simplify. apply G.set_of_graph_1 in H0. apply S.mem_1 in H0. rewrite H in H0. inversion H0.
+  - inversion H1; subst; simpl in *.
+    + destruct H2. destruct H2. destruct H2. inversion H2; subst. rewrite T.singleton_2 in H5. subst.
+      simplify. left. destruct (S.mem x(S.remove x remain_d)) eqn : ?. exfalso. eapply remove_eq. apply Heqb.
+      reflexivity.
+    + destruct H2. destruct H2. destruct H2. inversion H2; subst. apply T.add_child_6 in H5. destruct H5.
+      * destruct IHvalid_dfs_state. apply H0. simplify. destruct H6.
+        exists t. exists x1. split. reflexivity. apply H5. left. rewrite P2.FM.remove_b. simplify.
+        right. apply H6.
+      *  subst. simplify. left. destruct (S.mem x (S.remove x remain_d)) eqn : ?. exfalso.
+        eapply remove_eq. apply Heqb. reflexivity.
+    + simplify. right. rewrite P2.FM.remove_b. simplify.
+  - inversion H1; subst; simpl in *.
+    + destruct (O.eq_dec x v).
+      * unfold O.eq in e. subst. exists (T.singleton v). exists f. split. reflexivity.
+        apply T.singleton_2. reflexivity.
+      * destruct IHvalid_dfs_state. apply H0.
+        rewrite P2.FM.remove_b in H2. simplify.
+        -- simplify. destruct H7. destruct H2.
+        
+      assert (T.contains_vertex_1: forall 
+
+*)
+
+(**)
+Lemma stack_contains_parents: forall s g o x y,
+  valid_dfs_state s g o ->
+  white s x = false ->
+  In (x, Some y) (get_stack s) ->
+  (exists t f, get_forest s = t :: f /\ T.is_child t y x = true).
+Proof.
+  intros. unfold white in H0. induction H; subst; simpl in *.
+  - destruct o. destruct (G.contains_vertex g v). inversion H1. inversion H.
+    inversion H. inversion H1. inversion H1.
+  - inversion H2; subst; simpl in *.
+    assert (tl = nil). { remember (g0, T.singleton x0 :: f, f_times, M.add x0 (time + 1) d_times, time + 1, S.remove x0 remain_d, remain_f,
+       add_to_stack x0 g0 remain_d ++ (x0, None) :: tl) as s'.
+      pose proof (only_1_root s' g o x0). destruct H5. eapply step. apply H.
+      apply H2. subst; simpl. apply in_or_app. right. left. reflexivity. destruct H5; subst; simpl in *.
+      destruct tl. reflexivity. pose proof (app_inversion_2 _ (x0, None) x1 
+      (add_to_stack x0 g0 remain_d ++ (x0, None) :: nil) (p :: tl)). destruct H7. intro. inversion H7.
+      rewrite <- app_assoc. apply H5. rewrite H7 in H5. pose proof (app_inversion _ (x0, None) (x0, None)
+      (add_to_stack x0 g0 remain_d ++ (x0, None) :: x2) x1). destruct H8. rewrite <- app_assoc. apply H5.
+      rewrite <- H8 in H6. exfalso. apply (H6 x0). apply in_or_app. right. left. reflexivity. } subst.
+    + destruct (O.eq_dec x x0).
+      * unfold O.eq in e. subst. apply in_app_or in H1. destruct H1.
+        -- apply add_to_stack_neq in H1. contradiction.
+        -- simpl in H1. destruct H1. inversion H1. destruct H1.
+      * simplify. rewrite P2.FM.remove_neq_b in H5. apply in_app_or in H1.
+        destruct H1. apply only_add_yet_to_be_discovered in H1. 
+        remember (g0, f, f_times, d_times, time, remain_d, remain_f, st) as s'. rewrite H1 in H5. inversion H5.
+        simpl in H1. destruct H1; inversion H1. intro; subst. apply n. reflexivity.
+        apply in_app_or in H1. destruct H1. apply only_add_yet_to_be_discovered in H1.
+        remember(g0, f, f_times, d_times, time, remain_d, remain_f, st) as s'.
+        assert (S.mem x (get_remain_d s') = true) by (subst; simpl; assumption).
+        eapply not_f_if_not_d in H6. subst; simpl in *. rewrite H6 in H5. inversion H5. apply H.
+        destruct H1; inversion H1.
+    + destruct (pop_stack st remain_f) eqn : ?.
+      * simpl in H4. destruct (S.min_elt remain_d); inversion H4.
+      * simpl in *. rewrite <- H4 in Heqs. pose proof (pop_stack_app st remain_f).
+        destruct H5. destruct H5. destruct H5. subst. apply in_app_or in H1.
+        destruct H1. assert (A:=H1). apply add_to_stack_neq in H1.
+        apply only_add_yet_to_be_discovered in A. simplify. rewrite P2.FM.remove_neq_b in H5.
+        rewrite A in H5. inversion H5. intro. subst. apply H1. reflexivity.
+        remember (g0, t :: f, f_times, d_times, time, remain_d, remain_f, x1 ++ x2) as s'.
+        assert (S.mem x (get_remain_d s') = true) by (subst; simpl; assumption).
+        eapply not_f_if_not_d in H7. subst; simpl in *. rewrite H7 in H5. inversion H5. subst. apply H.
+        simplify.
+        -- destruct (O.eq_dec x x0). unfold O.eq in e. subst. simpl in H1. destruct H1. inversion H1; subst.
+            exists (T.add_child t y x0). exists f. split. reflexivity. apply T.add_child_1.
+            
+        destruct (O.eq_dec x x0).
+        -- unfold O.eq in e. subst. simpl in H1.
+      * 
+
+
+ rewrite 
+
+ apply H0. apply in_app_or in H0. destruct H0. apply add_to_stack_adds_parent in H0. inversion H0; subst.
+        
+
+Lemma after_stack_gray: forall s g o v x y l1 l2 p,
+  valid_dfs_state s g o ->
+  gray s v = true ->
+  (l1 ++ (v,p) :: l2 = get_stack s /\ forall p', ~In(v, p') l1) ->
+  v <> x ->
+  In (x,y) l1 ->
+  (exists t f, get_forest s = t :: f /\ T.is_descendent t v x = true).
+Proof.
+  intros. unfold gray in H0. simplify. induction H; subst; simpl in *.
+  - rewrite H4 in H5. inversion H5.
+  - inversion H1; subst; simpl in *.
+    + remember (g0, T.singleton x0 :: f, f_times, M.add x0 (time + 1) d_times, time + 1, S.remove x0 remain_d, remain_f,
+       add_to_stack x0 g0 remain_d ++ (x0, None) :: tl) as s'.
+      assert ( tl = nil). { pose proof (only_1_root s' g o x0). destruct H9. eapply step. apply H.
+      apply H1. subst; simpl. apply in_or_app. right. left. reflexivity. destruct H9; subst; simpl in *.
+      destruct tl. reflexivity. pose proof (app_inversion_2 _ (x0, None) x1 
+      (add_to_stack x0 g0 remain_d ++ (x0, None) :: nil) (p0 :: tl)). destruct H11. intro. inversion H11.
+      rewrite <- app_assoc. apply H9. rewrite H11 in H9. pose proof (app_inversion _ (x0, None) (x0, None)
+      (add_to_stack x0 g0 remain_d ++ (x0, None) :: x2) x1). destruct H12. rewrite <- app_assoc. apply H9.
+      rewrite <- H12 in H10. exfalso. apply (H10 x0). apply in_or_app. right. left. reflexivity. }
+      subst. destruct (O.eq_dec v x0).
+      * unfold O.eq in e. subst. destruct l2. apply app_inversion in H0. destruct H0. inversion H9; subst.
+         simpl in H0. unfold e.
+    
+only_1_root
+
+ destruct (O.eq_dec x x0).
+      * unfold O.eq in e. subst. 
+
+
+ destruct tl; simpl in *.
+      * assert (In (v, p) (add_to_stack x0 g0 remain_d ++ (x0, None) :: nil)).
+        rewrite <- H0. apply in_or_app. right. left. reflexivity. apply in_app_or in H8.
+        destruct H8. apply only_add_yet_to_be_discovered in H8. 
+
+
+
+ assert exists p', In (v p) ( 
+
+
+ destruct o. destruct (G.contains_ve
+
+Lemma top_of_stack_gray: forall s g o v x y tl,
+  valid_dfs_state s g o ->
+  gray s v = true ->
+  black s x = false ->
+  get_stack s = (x, y) :: tl ->
+  exists t f, get_forest s = t :: f /\ T.is_descendent t v x = true.
+Proof.
+  intros. unfold gray in H0. unfold black in H1. induction H.
+  - simpl in *. simplify. rewrite H3 in H. inversion H.
+  - inversion H3; subst; simpl in *.
+    + simplify.
+
+only_1_root
+
+
+ destruct o. destruc simpl in H1.
+  
+
 (*TODO: Parentheses Theorem - next big goal *)
 
 (*Discovered at definition*)
